formalize all ABI encodings

src/ABI.v
@@ -1,4 +1,4 @@
-Require Coder Ergs Pointer GPR MemoryManagement.
+Require Coder Ergs Pointer GPR MemoryManagement lib.BitsExt.
 
 Import ssreflect ssreflect.ssrfun ssreflect.ssrbool ssreflect.eqtype ssreflect.tuple zmodp.
 Import Core Common Coder Bool GPR Ergs Memory MemoryManagement Pointer.
@@ -16,138 +16,11 @@ The description from Rust VM implementation is described here:
 https://github.com/matter-labs/zkevm_opcode_defs/blob/v1.4.1/src/definitions/abi
 
 ## Fat pointers *)
-Module FatPointer.
-  Axiom ABI  : @coder u128 fat_ptr_nullable.
-
-  Definition decode_fat_ptr (w:u128) : option fat_ptr_nullable := ABI.(decode) w.
-
-  Definition decode_fat_ptr_word (w:word) : option (u128 * fat_ptr_nullable) :=
-    let (high128, low128) := split2 128 128 w in
-    match decode_fat_ptr low128 with
-    | Some fpn => Some (high128, fpn)
-    | _ => None
-    end
-  .
-
-  Definition decode_heap_ptr (w:word) : option (u224 * heap_ptr) :=
-    let (msbs, ofs) := split2 _ 32 w in
-    Some (msbs, mk_hptr ofs).
-
-  Definition encode_heap_ptr (h:heap_ptr) : option u32 :=
-    Some (hp_addr h)
-  .
-
-  Definition encode_heap_ptr_word (high224: u224) (h:heap_ptr) : option word :=
-    match encode_heap_ptr h with
-    | Some hpenc => Some (high224 ## hpenc)
-    | _ => None
-    end
-  .
-  Definition encode_fat_ptr (fp: fat_ptr_nullable) : u128 := ABI.(encode) fp.
-  Definition encode_fat_ptr_word (high_bytes: u128) (fp: fat_ptr_nullable) : word :=
-    high_bytes ## encode_fat_ptr fp.
-
-End FatPointer.
-
-
-(** ## Near call *)
-Module NearCall.
-
-  Record params: Type :=
-    mk_params {
-        ergs_passed: u32;
-      }.
-
-  Axiom ABI: @coder word params.
-
-End NearCall.
-
-
-(** ## Far returns *)
-Module FarRet.
-  Record params := mk_params {
-                           forwarded_memory :> fwd_memory
-                          }.
-  Axiom ABI: @coder word params.
-  Axiom ABI_decode_zero: ABI.(decode) word0 = Some (mk_params (ForwardNewFatPointer Heap span_empty)).
-End FarRet.
-
-(** ## Far call *)
-Module FarCall.
-  Import FatPointer.
-
-  Record params :=
-    mk_params {
-        fwd_memory: fwd_memory;
-        ergs_passed: ergs;
-        shard_id: shard_id;
-        constructor_call: bool;
-        to_system: bool;
-      }.
-
-  Axiom ABI: @coder word params.
-
-End FarCall.
-
-
-Module MetaParameters.
-
-  Record params :=
-    mk_params {
-        ergs_per_pubdata_byte: ergs;
-        heap_size: mem_address;
-        aux_heap_size: mem_address;
-        this_shard_id: shard_id;
-        caller_shard_id: shard_id;
-        code_shard_id: shard_id;
-      }.
-
-  Axiom ABI: @coder word params.
-
-End MetaParameters.
-
-Module PrecompileParameters.
-
-  Record params :=
-    mk_params
-      {
-        input_memory_offset: mem_address;
-        input_memory_length: mem_address;
-        output_memory_offset: mem_address;
-        output_memory_length: mem_address;
-        per_precompile_interpreted: u64;
-        memory_page_to_read: page_id;
-        memory_page_to_write: page_id;
-        precompile_interpreted_data: u64;
-      }.
-
-  Definition params_eqn (x y: params) : bool :=
-    (x.(input_memory_offset) == y.(input_memory_offset)) &&
-      (x.(input_memory_length) == y.(input_memory_length)) &&
-      (x.(output_memory_offset) == y.(output_memory_offset)) &&
-      (x.(output_memory_length) == y.(output_memory_length)) &&
-      (x.(per_precompile_interpreted) == y.(per_precompile_interpreted)) &&
-      (x.(memory_page_to_read) == y.(memory_page_to_read)) &&
-      (x.(memory_page_to_write) == y.(memory_page_to_write)) &&
-      (x.(precompile_interpreted_data) == y.(precompile_interpreted_data)).
-
-  Lemma params_eqnP : Equality.axiom params_eqn.
-  Proof.
-    move => x y.
-    unfold params_eqn.
-    destruct x,y =>//=.
-    repeat match goal with
-             [ |- context [(?x == ?y)] ] =>
-               let Hf := fresh "H" in
-               destruct (x == y) eqn: Hf; try rewrite Hf
-           end =>//=; constructor; auto;
-      repeat match goal with [ H: (?x == ?y) = true |- _] => move: H => /eqP -> end;
-      try injection; intros; subst;
-      repeat match goal with [ H: (?x == ?x) = false |- _] => rewrite eq_refl in H end =>//=.
-    - constructor.
-  Qed.
-  Canonical params_eqMixin := EqMixin params_eqnP.
-  Canonical params_eqType := Eval hnf in EqType _ params_eqMixin.
-  Axiom ABI: @coder word params.
-
-End PrecompileParameters.
+Require Export
+  ABI.FatPointerABI
+  ABI.MetaParametersABI
+  ABI.PrecompileParametersABI
+  ABI.NearCallABI
+  ABI.FarRetABI
+  ABI.FarCallABI
+.
