src/ABI/FarCallABI.v
@@ -1,0 +1,179 @@
+Require Coder Ergs MemoryManagement Pointer lib.BitsExt ABI.FatPointerABI ABI.ForwardPageTypesABI.
+
+Import ssreflect ssreflect.ssrfun ssreflect.eqtype ssreflect.tuple.
+Import Arith Core Common Coder Ergs Memory MemoryManagement Pointer lib.BitsExt FatPointerABI ForwardPageTypesABI.
+
+Record params :=
+  mk_params {
+      fwd_memory: fwd_memory;
+      ergs_passed: ergs;
+      shard_id: shard_id;
+      constructor_call: bool;
+      to_system: bool;
+    }.
+
+
+Record params_layout :=
+  mk_params_layout {
+      raw_to_system_bool: u8;
+      raw_constructor_call_bool: u8;
+      raw_shard_id: u8;
+      raw_memory_forwarding_type_enum : u8;
+      raw_ergs_passed: u32;
+      (*raw_reserved: u64; *)
+      raw_fat_ptr_layout: fat_ptr_layout;
+    }.
+
+Section BinaryCoder.
+  Open Scope ZMod_scope.
+  Definition encode_bin : @encoder word params_layout :=
+    fun params =>
+      match params with
+       | mk_params_layout to_system8 constructor_call8 shard_id8 memory_forwarding_type8 ergs_passed32 (* reserved64 *) fat_ptr_layout128 =>
+          match FatPointerABI.encode_bin fat_ptr_layout128 with
+          | Some ptr_encoded128 => Some (
+                                      to_system8 ## constructor_call8 ## shard_id8 ## memory_forwarding_type8 ##
+                                        ergs_passed32 ##
+                                        zero64 ##
+                                        ptr_encoded128)
+          | None => None
+          end
+      end
+  .
+
+
+  Definition decode_bin : @decoder word params_layout :=
+    fun w =>
+      let to_system : u8 := w { 256-8, 256 } in
+      let constructor_call : u8 := w { 256 - 2*8, 256 - 8 }  in
+      let shard_id : u8 := w { 256 - 3*8, 256 - 2*8 }  in
+      let memory_forwarding_type : u8 := w { 256 - 4*8, 256 - 3*8 }  in
+      let ergs_passed : u32 := w { 256 - 2*32, 256 - 32 }  in
+      let ptr : option fat_ptr_layout := FatPointerABI.decode_bin (low 128 w) in
+      match ptr with
+      | Some ptr => Some (mk_params_layout to_system constructor_call shard_id memory_forwarding_type ergs_passed ptr )
+      | None => None
+      end.
+
+
+  Theorem binary_coder_revertible: revertible decode_bin encode_bin.
+  Proof.
+    unfold revertible, encode_bin, decode_bin.
+    move => [s c sh mf es fpe] encoded.
+    move: (bits_size s) (bits_size c) (bits_size sh) (bits_size mf) (bits_size es) (bits_size encoded).
+    move => bits_size0 bits_size1 bits_size2 bits_size3 bits_size4 bits_size5.
+    case_eq (FatPointerABI.encode_bin fpe); last by discriminate.
+    {
+      inversion 2.
+      replace (low 128 _) with u.
+      {
+        move: (bits_size u) => bits_size6.
+        move: H => /FatPointerABI.fat_ptr_bin_revertible ->.
+        do 2 f_equal; by bits_solve_subranges.
+      }
+      {
+        unfold subrange, subrange_len; apply /eqP; rewrite -val_eqE.
+        move : (bits_size u) => bits_size6.
+        by rewrite low_val !take_cat; bits_solve_size; rewrite cats0.
+      }
+    }
+  Qed.
+
+
+  Definition coder_binary : @coder word params_layout :=
+    mk_coder decode_bin encode_bin binary_coder_revertible.
+
+End BinaryCoder.
+
+Section LayoutCoder.
+
+  Definition encode_layout: @encoder params_layout params :=
+fun params =>
+  match params with
+  | mk_params (ForwardExistingFatPointer fptr) ergs_passed shard_id constructor_call to_system =>
+      match FatPointerABI.encode_layout fptr with
+        | Some ptr_layout =>
+            Some
+              {|
+                raw_to_system_bool:= if to_system then # 1 else # 0;
+                raw_constructor_call_bool := if constructor_call then # 1 else # 0;
+                raw_shard_id := shard_id;
+                raw_memory_forwarding_type_enum := FarCallForwardPageType.ForwardFatPointer;
+                raw_ergs_passed:= ergs_passed;
+                (*raw_reserved: u64; *)
+                raw_fat_ptr_layout:= ptr_layout;
+              |}
+      | None => None
+      end
+  | mk_params (ForwardNewFatPointer heap_variant span) ergs_passed shard_id constructor_call to_system =>
+      Some
+        {|
+          raw_to_system_bool:= if to_system then # 1 else # 0;
+          raw_constructor_call_bool := if constructor_call then # 1 else # 0;
+          raw_shard_id := shard_id;
+          raw_memory_forwarding_type_enum := data_page_type_to_u8 heap_variant;
+          raw_ergs_passed := ergs_passed;
+          (*raw_reserved: u64; *)
+          raw_fat_ptr_layout:= {|
+                                start := span.(s_start);
+                                length := span.(s_length);
+                                page := zero32;
+                                offset := zero32;
+                              |};
+        |}
+  end.
+
+  Definition decode_layout: @decoder params_layout params :=
+    fun layout =>
+      match layout with
+      | mk_params_layout raw_to_system_bool raw_constructor_call_bool raw_shard_id raw_memory_forwarding_type_enum raw_ergs_passed raw_fat_ptr_layout =>
+          match fwd_memory_adapter raw_memory_forwarding_type_enum raw_fat_ptr_layout with
+          | Some fwd_memory_value => Some (
+                                        {|
+                                          fwd_memory := fwd_memory_value;
+                                          ergs_passed := raw_ergs_passed;
+                                          shard_id := raw_shard_id;
+                                          constructor_call := raw_constructor_call_bool != zero8;
+                                          to_system := raw_to_system_bool != zero8;
+                                        |})
+          | None => None
+          end
+      end
+  .
+
+  Theorem layout_coding_revertible: revertible decode_layout encode_layout.
+    unfold revertible.
+    unfold revertible, decode_layout, encode_layout, fwd_memory_adapter.
+    move => [fwd_memory ergs_passed shard_id constructor_call to_system encoded].
+    case_eq fwd_memory.
+    { (* Existing fatptr *)
+      move => p H. subst.
+      case_eq (FatPointerABI.encode_layout p); last by [].
+      {
+        intros f.
+        move /FatPointerABI.layout_coding_revertible.
+        intros Hptr.
+        inversion_clear 1.
+        rewrite Hptr.
+        by destruct constructor_call, to_system.
+      }
+    }
+    {
+      intros heap_var s H.
+      inversion 1.
+      subst encoded.
+     simpl.
+     repeat f_equal =>//=; try by destruct constructor_call, to_system.
+     clear H0.
+     {
+       unfold span_of. destruct heap_var;
+       repeat f_equal =>//=; try by destruct constructor_call, to_system, s.
+     }
+    }
+  Qed.
+
+  Definition coder_layout := mk_coder decode_layout encode_layout layout_coding_revertible.
+
+End LayoutCoder.
+
+Definition coder := coder_compose coder_binary coder_layout.
