src/ABI/FatPointerABI.v
@@ -1,0 +1,165 @@
+Require Coder Pointer lib.BitsExt.
+
+Import ssreflect ssreflect.ssrfun ssreflect.eqtype ssreflect.tuple.
+Import Core Common Coder Pointer lib.BitsExt.
+
+(** Record [%fat_ptr_layout] displays the memory layout of a 128-bit fat pointer.*)
+Record fat_ptr_layout := mk_fat_ptr_layout {
+                              length: u32;
+                              start: u32;
+                              page: u32;
+                              offset: u32;
+                            }.
+Definition null_fat_ptr_layout := mk_fat_ptr_layout zero32 zero32 zero32 zero32.
+
+Section LayoutCoder.
+  (** Functions [%encode_layout] and [%decode_layout] formalize the encoding of
+  a [%fat_ptr_nullable] to [%fat_ptr_layout]. *)
+  Definition encode_layout : @encoder fat_ptr_layout fat_ptr_nullable :=
+    fun fp : fat_ptr_nullable =>
+      match fp with
+      | NullPtr => Some null_fat_ptr_layout
+      | NotNullPtr (mk_fat_ptr p (mk_ptr (mk_span s l) ofs)) =>
+          if (p == 0)  || (p >= 2^32) then None else
+            Some (mk_fat_ptr_layout l s (# p) ofs)
+      end.
+
+  Definition decode_layout : @decoder fat_ptr_layout fat_ptr_nullable :=
+    fun w: fat_ptr_layout =>
+      match w with
+      | mk_fat_ptr_layout length start page offset =>
+          if page == zero32 then Some NullPtr else
+            Some (NotNullPtr {|
+                      fp_page := toNat page;
+                      fp_ptr := {|
+                                 p_span := mk_span start length;
+                                 p_offset := offset;
+                               |}
+                    |})
+      end.
+
+  Theorem layout_coding_revertible: revertible decode_layout encode_layout.
+  Proof.
+    move => [|[page [[start length] ofs]]]; first by inversion 1.
+    move => [length' start' page' ofs'] //=.
+    case_eq (page == 0) => Hva2 ; first by inversion_clear 1.
+    simpl.
+    case_eq (2^32 <= page); first by inversion 1.
+    inversion 2.
+    subst.
+    have Hpagelt: page < 2^32.
+    rewrite ltnNge.
+    by move: H ; case (2^32 <= page).
+    have Hpage: # ( page) == zero32 = false.
+    {
+      symmetry; rewrite -Hva2.
+      by apply properties.fromNatBounded_eq.
+    }
+    {
+      rewrite Hpage.
+      repeat f_equal.
+      by apply properties.toNat_fromNatBounded.
+    }
+  Qed.
+
+  Definition fat_ptr_layout_coder : @Coder.coder fat_ptr_layout fat_ptr_nullable
+    := mk_coder decode_layout encode_layout layout_coding_revertible.
+
+End LayoutCoder.
+
+Section BinaryCoder.
+  #[local] Open Scope ZMod_scope.
+
+  Definition encode_bin: @encoder u128 fat_ptr_layout :=
+    fun fp: fat_ptr_layout =>
+      match fp with
+      | mk_fat_ptr_layout length start page offset =>
+          Some (length ## start ## page ## offset)
+      end.
+
+  Definition decode_bin : @decoder u128 fat_ptr_layout :=
+    fun w: u128 =>
+      let length := w { 3*32, 4*32 } in
+      let start  := w { 2*32, 3*32 } in
+      let page   := w { 32, 2*32} in
+      let offset := w { 0, 32 } in
+      Some (mk_fat_ptr_layout length start page offset).
+
+  Lemma fat_ptr_bin_revertible: revertible decode_bin encode_bin.
+  Proof.
+    move => [a b p d] w.
+    have: (size a = 32) by apply /eqP; case a.
+    have: (size b = 32) by apply /eqP; case b.
+    have: (size p = 32) by apply /eqP; case p.
+    have: (size d = 32) by apply /eqP; case d.
+    move => Hd Hp Hb Ha.
+    inversion_clear 1.
+    unfold encode_bin, decode_bin.
+    f_equal.
+    unfold subrange, subrange_len.
+    f_equal; apply /eqP.
+    {
+      rewrite -val_eqE high_val low_val.
+      simpl.
+      have H1: (size (((d ++ p) ++ b) ++ a) = 128) by rewrite! size_cat Hd Hp Hb Ha.
+      have H2: (size ((d ++ p) ++ b) = 96) by rewrite! size_cat Hd Hp Hb.
+      replace (3 * 32 + 32)%nat with (size (((d ++ p) ++ b) ++ a)).
+      by rewrite take_size drop_size_cat.
+    }
+    {
+      by rewrite properties.low_catB properties.high_catB.
+    }
+    {
+      replace (a ## b ## p ## d) with ((a ## b) ## (p ## d));
+        first by rewrite properties.low_catB properties.high_catB.
+      apply /eqP; unfold eq_op =>//=.
+      by rewrite catA.
+    }
+    {
+      replace (a ## b ## p ## d) with ((a ## b ## p) ## d);
+        first by rewrite properties.low_catB.
+      apply /eqP; unfold eq_op =>//=.
+      by rewrite! catA.
+    }
+  Qed.
+
+  Definition binary_coder: @Coder.coder u128 fat_ptr_layout :=
+    mk_coder decode_bin encode_bin fat_ptr_bin_revertible.
+End BinaryCoder.
+
+Section ComposedCoder.
+  Definition ABI : @Coder.coder u128 fat_ptr_nullable :=
+    coder_compose binary_coder fat_ptr_layout_coder.
+
+
+  Definition decode_fat_ptr (w:u128) : option fat_ptr_nullable := ABI.(decode) w.
+
+  Definition decode_fat_ptr_word (w:word) : option (u128 * fat_ptr_nullable) :=
+    let (high128, low128) := split2 128 128 w in
+    match decode_fat_ptr low128 with
+    | Some fpn => Some (high128, fpn)
+    | _ => None
+    end
+  .
+
+  Definition decode_heap_ptr (w:word) : option (u224 * heap_ptr) :=
+    let (msbs, ofs) := split2 _ 32 w in
+    Some (msbs, mk_hptr ofs).
+
+  Definition encode_heap_ptr (h:heap_ptr) : option u32 :=
+    Some (hp_addr h)
+  .
+
+  Definition encode_heap_ptr_word (high224: u224) (h:heap_ptr) : option word :=
+    match encode_heap_ptr h with
+    | Some hpenc => Some (high224 ## hpenc)
+    | _ => None
+    end
+  .
+  Definition encode_fat_ptr (fp: fat_ptr_nullable) : option u128 := ABI.(encode) fp.
+  Definition encode_fat_ptr_word (high_bytes: u128) (fp: fat_ptr_nullable) : option word :=
+    match encode_fat_ptr fp with
+    | Some enc => Some (high_bytes ## enc)
+    | _ => None
+    end.
+End ComposedCoder.
