src/ABI/ForwardPageTypesABI.v
@@ -1,0 +1,34 @@
+Require Coder Ergs MemoryManagement Pointer lib.BitsExt ABI.FatPointerABI.
+
+Import ssreflect ssreflect.ssrfun ssreflect.eqtype ssreflect.tuple.
+Import Arith Core Common Coder Ergs Memory MemoryManagement Pointer lib.BitsExt FatPointerABI.
+
+Module FarCallForwardPageType.
+  Definition UseHeap : u8 := # 0.
+  Definition ForwardFatPointer : u8 := # 1.
+  Definition UseAuxHeap : u8 := # 2.
+  (* other u8 values are mapped to UseHeap. *)
+End FarCallForwardPageType.
+
+Definition data_page_type_to_u8 (t:data_page_type) : u8 :=
+  match t with
+  | Heap => FarCallForwardPageType.UseHeap
+  | AuxHeap =>FarCallForwardPageType.UseAuxHeap
+  end.
+
+Definition span_of (fp: fat_ptr_layout) : span :=
+  mk_span fp.(start) fp.(length).
+
+Definition fwd_memory_adapter (fwd_type: u8) (raw_fat_ptr_layout: fat_ptr_layout) : option MemoryManagement.fwd_memory:=
+  if fwd_type == FarCallForwardPageType.ForwardFatPointer then
+    option_map ForwardExistingFatPointer
+      (FatPointerABI.decode_layout raw_fat_ptr_layout)
+  else
+    let span := span_of raw_fat_ptr_layout in
+    Some (
+        if fwd_type == FarCallForwardPageType.UseAuxHeap then
+          ForwardNewFatPointer AuxHeap span
+        else (* Heap or a default option *)
+          ForwardNewFatPointer Heap span
+      )
+.
