src/ABI/MetaParametersABI.v
@@ -1,0 +1,136 @@
+Require Coder Ergs MemoryManagement Pointer lib.BitsExt.
+
+Import ssreflect ssreflect.ssrfun ssreflect.eqtype ssreflect.tuple.
+Import Arith Core Common Coder Ergs Memory MemoryManagement Pointer lib.BitsExt.
+
+Record params :=
+  mk_params {
+      ergs_per_pubdata_byte: ergs;
+      heap_size: mem_address;
+      aux_heap_size: mem_address;
+      this_shard_id: shard_id;
+      caller_shard_id: shard_id;
+      code_shard_id: shard_id;
+    }.
+
+Record params_layout :=
+  mk_params_layout {
+      (* reserved: u8 *)
+      l_code_shard_id : u8;
+      l_caller_shard_id : u8;
+      l_this_shard_id : u8;
+     (* reserved: u96 *)
+      l_aux_heap_size : u32;
+      l_heap_size : u32;
+      (* reserved: u32 *)
+      l_ergs_per_pubdata_byte: u32;
+  }.
+
+Section BinaryCoder.
+  #[local] Open Scope ZMod_scope.
+  Context (zero96 : BITS 96 := # 0).
+
+  Definition encode_bin : @encoder word params_layout :=
+    fun layout =>
+      match layout with
+      | mk_params_layout
+          l_code_shard_id8
+          l_caller_shard_id8
+          l_this_shard_id8
+          l_aux_heap_size32
+          l_heap_size32
+          l_ergs_per_pubdata_byte32
+        => Some (
+              zero8 ## l_code_shard_id8 ## l_caller_shard_id8 ## l_this_shard_id8 ## zero96 ## l_aux_heap_size32 ## l_heap_size32 ## zero32 ## l_ergs_per_pubdata_byte32)
+      end.
+
+  Definition decode_bin: @decoder word params_layout :=
+    fun w =>
+      Some {|
+          (* reserved: u8 *)
+          l_code_shard_id := w { 256 - 2*8 , 256 - 8} ;
+          l_caller_shard_id := w {256 - 3 * 8, 256 - 2 * 8};
+          l_this_shard_id := w {256 - 4 * 8, 256 - 3 * 8};
+          (* reserved: u96 *)
+          l_aux_heap_size := w { 3 * 32, 4 * 32 };
+          l_heap_size := w { 2 * 32, 3 * 32 };
+          (* reserved: u32 *)
+          l_ergs_per_pubdata_byte:= w { 0, 32 };
+        |}.
+
+
+  Theorem binary_coder_revertible: revertible decode_bin encode_bin.
+  Proof.
+     unfold revertible, decode_bin, encode_bin.
+     destruct obj.
+     inversion 1.
+     subst.
+     move :
+       (bits_size l_code_shard_id0)
+         (bits_size l_caller_shard_id0)
+         (bits_size l_this_shard_id0)
+         (bits_size l_aux_heap_size0)
+         (bits_size l_heap_size0)
+         (bits_size l_ergs_per_pubdata_byte0)
+         (bits_size zero96)
+         (bits_size zero8)
+         (bits_size zero32)
+     .
+     move =>bits_size bits_size0 bits_size1 bits_size2 bits_size3 bits_size4 bits_size5 bits_size6 bits_size7.
+     repeat f_equal; try by bits_solve_subranges.
+     {
+       unfold subrange, subrange_len; apply /eqP; rewrite -val_eqE.
+       repeat rewrite high_val; repeat rewrite low_val.
+       rewrite drop0.
+       repeat (rewrite take_cat; bits_solve_size; simpl).
+       by rewrite take_size_cat.
+     }
+  Qed.
+
+  Definition binary_coder := mk_coder decode_bin encode_bin binary_coder_revertible.
+End BinaryCoder.
+
+
+Section LayoutCoder.
+
+Definition decode_layout : @decoder params_layout params :=
+  fun layout =>
+    match layout with
+    | mk_params_layout l_code_shard_id l_caller_shard_id l_this_shard_id l_aux_heap_size l_heap_size
+        l_ergs_per_pubdata_byte => Some
+                                    {|
+                                      ergs_per_pubdata_byte := l_ergs_per_pubdata_byte;
+                                      heap_size := l_heap_size;
+                                      aux_heap_size := l_aux_heap_size;
+                                      this_shard_id := l_this_shard_id;
+                                      caller_shard_id := l_caller_shard_id;
+                                      code_shard_id := l_code_shard_id;
+                                    |}
+    end.
+
+
+Definition encode_layout : @encoder params_layout params :=
+  fun params =>
+    match params with
+    | mk_params ergs_per_pubdata_byte heap_size aux_heap_size this_shard_id caller_shard_id code_shard_id => Some
+                                    {|
+                                      l_ergs_per_pubdata_byte := ergs_per_pubdata_byte;
+                                      l_heap_size := heap_size;
+                                      l_aux_heap_size := aux_heap_size;
+                                      l_this_shard_id := this_shard_id;
+                                      l_caller_shard_id := caller_shard_id;
+                                      l_code_shard_id := code_shard_id;
+                                    |}
+    end.
+
+Theorem layout_coder_revertible: revertible decode_layout encode_layout.
+Proof.
+  unfold revertible, encode_layout, decode_layout.
+  move => [ergs_per_pubdata_byte0 heap_size0 aux_heap_size0 this_shard_id0 caller_shard_id0 code_shard_id0].
+  by inversion_clear 1.
+Qed.
+
+  Definition layout_coder := mk_coder decode_layout encode_layout layout_coder_revertible.
+End LayoutCoder.
+
+Definition coder := coder_compose binary_coder layout_coder.
