src/ABI/NearCallABI.v
@@ -1,0 +1,24 @@
+Require Coder Ergs Memory.
+
+Import ssreflect.
+Import Types Core Coder Ergs Memory.
+
+Record params: Type :=
+  mk_params {
+      ergs_passed: u32;
+    }.
+
+Definition encode : params -> option u32 := fun p => Some p.(ergs_passed).
+Definition decode : u32 -> option params := fun u => Some (mk_params u).
+
+Definition encode_word (p:params) (high224: u224) : option word :=
+  option_map (fun encoded => high224 ## encoded) (encode p).
+
+Definition decode_word (w:word) : option (u224 * params) :=
+  option_map (fun decoded => (@high 224 32 w, decoded)) (decode (low 32 w)).
+
+Definition coder : @coder u32 params.
+refine (mk_coder decode encode _).
+unfold revertible, encode, decode.
+by move => []; inversion 1.
+Defined.
