src/ABI/PrecompileParametersABI.v
@@ -1,0 +1,53 @@
+Require Coder Memory lib.BitsExt.
+
+Import ssreflect ssreflect.ssrfun ssreflect.eqtype ssreflect.tuple.
+Import Core Common Coder Memory lib.BitsExt.
+
+Record params :=
+  mk_params
+    {
+      input_memory_offset: mem_address;
+      input_memory_length: mem_address;
+      output_memory_offset: mem_address;
+      output_memory_length: mem_address;
+      per_precompile_interpreted: u64;
+      memory_page_to_read: page_id;
+      memory_page_to_write: page_id;
+      precompile_interpreted_data: u64;
+    }.
+
+(* begin details: equality *)
+
+Definition params_eqn (x y: params) : bool :=
+  (x.(input_memory_offset) == y.(input_memory_offset)) &&
+    (x.(input_memory_length) == y.(input_memory_length)) &&
+    (x.(output_memory_offset) == y.(output_memory_offset)) &&
+    (x.(output_memory_length) == y.(output_memory_length)) &&
+    (x.(per_precompile_interpreted) == y.(per_precompile_interpreted)) &&
+    (x.(memory_page_to_read) == y.(memory_page_to_read)) &&
+    (x.(memory_page_to_write) == y.(memory_page_to_write)) &&
+    (x.(precompile_interpreted_data) == y.(precompile_interpreted_data)).
+
+Lemma params_eqnP : Equality.axiom params_eqn.
+Proof.
+  move => x y.
+  unfold params_eqn.
+  destruct x,y =>//=.
+  repeat match goal with
+           [ |- context [(?x == ?y)] ] =>
+             let Hf := fresh "H" in
+             destruct (x == y) eqn: Hf; try rewrite Hf
+         end =>//=; constructor; auto;
+    repeat match goal with [ H: (?x == ?y) = true |- _] => move: H => /eqP -> end;
+    try injection; intros; subst;
+    repeat match goal with [ H: (?x == ?x) = false |- _] => rewrite eq_refl in H end =>//=.
+  - constructor.
+Qed.
+
+Canonical params_eqMixin := EqMixin params_eqnP.
+Canonical params_eqType := Eval hnf in EqType _ params_eqMixin.
+(* end details *)
+
+
+
+Axiom ABI: @coder word params.
