src/lib/BitsExt.v
@@ -1,0 +1,42 @@
+From mathcomp Require Import ssreflect eqtype seq tuple ssrbool.
+
+From Bits Require Import spec bits tuple nat.
+From EraVM Require Arith.
+
+Import ssreflect.eqtype ssreflect.tuple Arith.
+
+Lemma low_val n m b: val (@low n m b) = take m (val b).
+elim: m n b.
+- by intros; rewrite take0.
+- move => //= n H n0 b.
+  case /tupleP: b => x t //=.
+  rewrite theadE.
+  f_equal. by rewrite tuple.beheadCons.
+Qed.
+
+Lemma high_val n m b: val (@high n m b) = drop m (val b).
+Proof.
+    elim: m n b.
+  - by intros; rewrite drop0.
+  - move => //= n H n0 b.
+    case /tupleP: b => x t //=.
+    by rewrite tuple.beheadCons.
+Qed.
+
+Lemma val_catB n m (a:BITS n) (b:BITS m): val (a ## b) = b ++ a.
+ Proof. by done. Qed.
+
+ Lemma bits_size {n} (b:BITS n): size b = n.
+   destruct b. simpl.
+   pose proof (@eqP ssrnat.nat_eqType (size tval) n).
+   inversion H; by [| rewrite i in H0].
+ Qed.
+
+ Ltac bits_subst_size:= repeat match goal with | [H : size ?x = _ |- context [size ?x]] => rewrite H end.
+ Ltac bits_solve_size := rewrite !size_cat; bits_subst_size.
+ Ltac bits_solve_subranges :=
+   unfold subrange, subrange_len; apply /eqP; rewrite -val_eqE;
+   repeat rewrite high_val; repeat rewrite low_val;
+   repeat (rewrite take_cat; bits_solve_size; simpl);
+   repeat (rewrite drop_cat; bits_solve_size; simpl);
+     by repeat try do [rewrite !take0| rewrite! drop0 | rewrite! cats0 | rewrite! take_oversize| rewrite! take_size_cat | bits_subst_size].
