src/lib/Show.v
@@ -1,0 +1,67 @@
+From ExtLib Require Import ExtLib Show.
+From Bits Require Import spec.
+Require Pointer.
+
+Import Coq.Strings.String Bool Ascii Show.
+Import ShowNotation.
+Import Pointer Types.
+
+Section ShowInstances.
+
+  Open Scope show_scope.
+  Global Instance bits_Show : forall n, Show (BITS n):=
+    { show b := toHex b }.
+
+  Compute to_string zero32.
+  #[local]
+    Open Scope string.
+  #[global]
+    Instance span_Show : Show span :=
+    { show s :=
+        match s with
+        | mk_span s l => ("[" ++ to_string s ++ ", " ++ to_string s ++ " + " ++ to_string l ++ ")")%string
+        end
+    }.
+
+  #[global]
+    Instance free_ptr_Show : Show free_ptr :=
+    { show p :=
+        match p with
+        | mk_ptr s ofs => "offset " ++ to_string ofs ++ " in " ++ to_string s
+        end
+    }.
+
+  #[global]
+    Instance fat_ptr_Show : Show fat_ptr :=
+    { show p :=
+        match p with
+        | mk_fat_ptr page fp => "fat ptr to page " ++ to_string page ++ ", " ++ to_string fp
+        end
+    }.
+
+  #[global]
+    Instance fat_ptr_nullable_Show : Show fat_ptr_nullable :=
+    { show p :=
+        match p with
+        | NullPtr => "NullPtr"
+        | NotNullPtr ptr => to_string ptr
+        end
+    }.
+
+
+  #[global]
+    Instance option_Show {T} `{Show T}: Show (option T) :=
+    { show o :=
+        match o with
+        | Some e=> show e
+        | None => "None"
+        end
+    }.
+(* Examples:
+
+```
+Compute (to_string (FatPointerABI.ABI.(decode) (zero32 ## zero32 ## @fromNat 32 1  ## zero32))).
+Compute to_string (NotNullPtr (mk_fat_ptr #(1) (mk_ptr (mk_span zero32 #(92)) zero32))).
+```
+ *)
+End ShowInstances.
