src/sem/Context.v
@@ -3,7 +3,7 @@ From RecordUpdate Require Import RecordSet.
 Require SemanticCommon.
 
 Import Addressing ABI Bool Coder Core Common Predication Ergs CallStack Memory MemoryOps isa.CoreSet State
-  Addressing.Coercions PrimitiveValue SemanticCommon RecordSetNotations ABI.MetaParameters.
+  Addressing.Coercions PrimitiveValue SemanticCommon RecordSetNotations ABI.MetaParametersABI.
 
 Section ContextDefinitions.
 (** # ContextThis
