src/sem/PrecompileCall.v
@@ -3,7 +3,7 @@ From RecordUpdate Require Import RecordSet.
 Require SemanticCommon Precompiles.
 
 Import Addressing ABI Bool Common Coder Predication Ergs CallStack Event Memory MemoryOps isa.CoreSet State
-  Addressing.Coercions PrimitiveValue SemanticCommon RecordSetNotations MetaParameters ABI.PrecompileParameters.
+  Addressing.Coercions PrimitiveValue SemanticCommon RecordSetNotations PrecompileParametersABI.
 
 Section PrecompileCallDefinition.
   Open Scope ZMod_scope.
